die due to debrujin indices

language_formalisation/substitution/substitution.v
@@ -1,5 +1,5 @@
-Add LoadPath "C:\Users\Ziga\Documents\Ziga_podatki\PHD\language_formalisation\syntax".
-(* Add LoadPath "E:\Ziga_Podatki\faks\PHD\language_formalisation\syntax". *)
+(* Add LoadPath "C:\Users\Ziga\Documents\Ziga_podatki\PHD\language_formalisation\syntax". *)
+Add LoadPath "E:\Ziga_Podatki\faks\PHD\language_formalisation\syntax".
 Require Export syntax Arith.
 Require Import Le Compare_dec.
 
@@ -7,41 +7,34 @@ Module Sub.
 
 Fixpoint v_shift (v : val) d (cut : nat) :=
 match v with
-| Var (x, n) => 
-    if cut <=? n then Var (x, n + d) else Var (x, n)
+| Var (x, n) => if cut <=? n then Var (x, n + d) else Var (x, n)
 | Unit => Unit
 | Int n => Int n
 | Inl v' => Inl (v_shift v' d cut)
 | Inr v' => Inr (v_shift v' d cut)
 | Pair v1 v2 => Pair (v_shift v1 d cut) (v_shift v2 d cut)
 | Fun x c => Fun x (c_shift c d (cut+1))
-| Handler x c_ret h =>
-    Handler x (c_shift c_ret d (cut+1)) (h_shift h d cut)
+| Handler x c_ret h => Handler x (c_shift c_ret d (cut+1)) (h_shift h d cut)
 end
 with c_shift (c : comp) d (cut : nat) :=
 match c with
 | Ret v => Ret (v_shift v d cut)
 | Absurd v => Absurd (v_shift v d cut)
-| ΠMatch v x y c =>
-    ΠMatch (v_shift v d cut) x y (c_shift c d (cut+2))
+| ΠMatch v x y c => ΠMatch (v_shift v d cut) x y (c_shift c d (cut+2))
 | ΣMatch v xl cl xr cr =>
     ΣMatch (v_shift v d cut)
       xl (c_shift cl d (cut+1))
       xr (c_shift cr d (cut+1))
 | App v1 v2 => App (v_shift v1 d cut) (v_shift v2 d cut)
-| Op op v_arg y c =>
-    Op op (v_shift v_arg d cut) y (c_shift c d (cut+1))
-| LetRec f x c1 c2 =>
-    LetRec f x (c_shift c1 d (cut+2)) (c_shift c2 d (cut+1))
-| DoBind x c1 c2 =>
-    DoBind x (c_shift c1 d cut) (c_shift c2 d (cut+1))
+| Op op v_arg y c => Op op (v_shift v_arg d cut) y (c_shift c d (cut+1))
+| LetRec f x c1 c2 => LetRec f x (c_shift c1 d (cut+2)) (c_shift c2 d (cut+1))
+| DoBind x c1 c2 => DoBind x (c_shift c1 d cut) (c_shift c2 d (cut+1))
 | Handle v c' => Handle (v_shift v d cut) (c_shift c' d cut)
 end
 with h_shift (h : hcases) d (cut : nat) :=
 match h with
 | CasesØ => CasesØ
-| CasesU h op x k c => 
-    CasesU (h_shift h d cut) op x k (c_shift c d (cut+2))
+| CasesU h op x k c => CasesU (h_shift h d cut) op x k (c_shift c d (cut+2))
 end.
 
 Fixpoint sub_shift (sub : nat * val) d :=
@@ -64,19 +57,16 @@ with c_negshift (c : comp) d (cut : nat) :=
 match c with
 | Ret v => Ret (v_negshift v d cut)
 | Absurd v => Absurd (v_negshift v d cut)
-| ΠMatch v x y c =>
-    ΠMatch (v_negshift v d cut) x y (c_negshift c d (cut+2))
+| ΠMatch v x y c => ΠMatch (v_negshift v d cut) x y (c_negshift c d (cut+2))
 | ΣMatch v xl cl xr cr =>
     ΣMatch (v_negshift v d cut)
       xl (c_negshift cl d (cut+1))
       xr (c_negshift cr d (cut+1))
 | App v1 v2 => App (v_negshift v1 d cut) (v_negshift v2 d cut)
-| Op op v_arg y c =>
-    Op op (v_negshift v_arg d cut) y (c_negshift c d (cut+1))
+| Op op v_arg y c => Op op (v_negshift v_arg d cut) y (c_negshift c d (cut+1))
 | LetRec f x c1 c2 =>
     LetRec f x (c_negshift c1 d (cut+2)) (c_negshift c2 d (cut+1))
-| DoBind x c1 c2 =>
-    DoBind x (c_negshift c1 d cut) (c_negshift c2 d (cut+1))
+| DoBind x c1 c2 => DoBind x (c_negshift c1 d cut) (c_negshift c2 d (cut+1))
 | Handle v c' => Handle (v_negshift v d cut) (c_negshift c' d cut)
 end
 with h_negshift (h : hcases) d (cut : nat) :=
@@ -105,42 +95,41 @@ with c_sub (c : comp) (sub : nat * val) :=
 match c with
 | Ret v => Ret (v_sub v sub)
 | Absurd v => Absurd (v_sub v sub)
-| ΠMatch v x y c =>
-    ΠMatch (v_sub v sub) x y (c_sub c (sub_shift sub 2))
+| ΠMatch v x y c => ΠMatch (v_sub v sub) x y (c_sub c (sub_shift sub 2))
 | ΣMatch v xl cl xr cr =>
     ΣMatch (v_sub v sub)
       xl (c_sub cl (sub_shift sub 1))
       xr (c_sub cr (sub_shift sub 1))
 | App v1 v2 => App (v_sub v1 sub) (v_sub v2 sub)
-| Op op v_arg y c =>
-    Op op (v_sub v_arg sub) y (c_sub c (sub_shift sub 1))
+| Op op v_arg y c => Op op (v_sub v_arg sub) y (c_sub c (sub_shift sub 1))
 | LetRec f x c1 c2 =>
-    LetRec f x 
-      (c_sub c1 (sub_shift sub 2))
-      (c_sub c2 (sub_shift sub 1))
-| DoBind x c1 c2 =>
-    DoBind x (c_sub c1 sub) (c_sub c2 (sub_shift sub 1))
+    LetRec f x (c_sub c1 (sub_shift sub 2)) (c_sub c2 (sub_shift sub 1))
+| DoBind x c1 c2 => DoBind x (c_sub c1 sub) (c_sub c2 (sub_shift sub 1))
 | Handle v c' => Handle (v_sub v sub) (c_sub c' sub)
 end
 with h_sub (h : hcases) (sub : nat * val) :=
 match h with
 | CasesØ => CasesØ
-| CasesU h op x k c => 
-    CasesU
-      (h_sub h sub) op x k (c_sub c (sub_shift sub 2))
+| CasesU h op x k c => CasesU (h_sub h sub) op x k (c_sub c (sub_shift sub 2))
 end.
 
 End Sub.
 
 (* Instantiates the outer binder, takes care of all the shifting. *)
-Definition v_sub_out (v:val) (v_s:val) :=
-  Sub.v_negshift (Sub.v_sub v (0, (Sub.v_shift v_s 1 0))) 1 0.
+Definition v_sub (v:val) (v_s:val) i :=
+  Sub.v_negshift (Sub.v_sub v (i, (Sub.v_shift v_s 1 i))) 1 i.
 
-Definition c_sub_out (c:comp) (v_s:val) :=
-  Sub.c_negshift (Sub.c_sub c (0, (Sub.v_shift v_s 1 0))) 1 0.
+Definition c_sub (c:comp) (v_s:val) i :=
+  Sub.c_negshift (Sub.c_sub c (i, (Sub.v_shift v_s 1 i))) 1 i.
 
-Definition h_sub_out (h:hcases) (v_s:val) :=
-  Sub.h_negshift (Sub.h_sub h (0, (Sub.v_shift v_s 1 0))) 1 0.
+Definition h_sub (h:hcases) (v_s:val) i :=
+  Sub.h_negshift (Sub.h_sub h (i, (Sub.v_shift v_s 1 i))) 1 i.
+
+Definition v_sub_out (v:val) (v_s:val) := v_sub v v_s 0.
+
+Definition c_sub_out (c:comp) (v_s:val) := c_sub c v_s 0.
+
+Definition h_sub_out (h:hcases) (v_s:val) := h_sub h v_s 0.
 
 Definition c_sub2_out (c:comp) v1 v0 :=
   (* 1 -> v1, 0 -> v0 *)
