language_formalisation/substitution/substitution_lemmas.v
@@ -1,9 +1,9 @@
-Add LoadPath "C:\Users\Ziga\Documents\Ziga_podatki\PHD\language_formalisation\substitution".
-Add LoadPath "C:\Users\Ziga\Documents\Ziga_podatki\PHD\language_formalisation\syntax".
-(* Add LoadPath "E:\Ziga_Podatki\faks\PHD\language_formalisation\substitution". *)
-(* Add LoadPath "E:\Ziga_Podatki\faks\PHD\language_formalisation\syntax". *)
+(* Add LoadPath "C:\Users\Ziga\Documents\Ziga_podatki\PHD\language_formalisation\substitution". *)
+(* Add LoadPath "C:\Users\Ziga\Documents\Ziga_podatki\PHD\language_formalisation\syntax". *)
+Add LoadPath "E:\Ziga_Podatki\faks\PHD\language_formalisation\substitution".
+Add LoadPath "E:\Ziga_Podatki\faks\PHD\language_formalisation\syntax".
 Require Export substitution syntax_lemmas.
-Require Import Arith Le PeanoNat.
+Require Import Arith Le.
 
 
 Lemma v_shift_shift n m cut (v:val) :
@@ -38,6 +38,7 @@ revert cut. induction h; intros cut; simpl; f_equal.
 reflexivity. apply IHh. apply c_shift_shift.
 }
 Qed.
+
 
 Lemma v_shift_makes_no_var v j:
   v_no_var_j (Sub.v_shift v 1 j) j
@@ -138,3 +139,372 @@ rewrite (v_shift_shift _ _ _) in H.
 assert (j+1+1=j+2) by omega. rewrite H0 in H. auto. omega.
 }
 Qed.
+
+Lemma h_shift_find_op_None h o i j :
+  find_op_case h o = None <-> find_op_case (Sub.h_shift h i j) o = None.
+Proof.
+constructor; intro; induction h; auto; simpl in *;
+destruct (o==o0) eqn:cmp; try discriminate; auto.
+Qed.
+
+Lemma h_shift_find_op_Some h o i j x k cop :
+  find_op_case h o = Some (x, k, cop) -> 
+  find_op_case (Sub.h_shift h i j) o = 
+    Some (x, k, (Sub.c_shift cop i (j+2))).
+Proof.
+intro; induction h.
++ simpl in H. discriminate.
++ simpl in *. destruct (o==o0) eqn:cmp. inv H. all: auto.
+Qed.
+
+
+
+(* needed for tmpl handling *)
+Lemma v_shift_comm_aux n i j d (v:val) :
+i >= j ->
+Sub.v_shift (Sub.v_shift v n i) d j = Sub.v_shift (Sub.v_shift v d j) n (i+d)
+
+with c_shift_comm_aux n i j d (c:comp) :
+i >= j ->
+Sub.c_shift (Sub.c_shift c n i) d j = Sub.c_shift (Sub.c_shift c d j) n (i+d)
+
+with h_shift_comm_aux n i j d (h:hcases) :
+i >= j ->
+Sub.h_shift (Sub.h_shift h n i) d j = Sub.h_shift (Sub.h_shift h d j) n (i+d).
+Proof.
+{
+intros cmp. induction v; simpl.
+{ 
+  clear v_shift_comm_aux c_shift_comm_aux h_shift_comm_aux.
+  destruct v as (x, dbi).
+  destruct (i<=?dbi) eqn:cmpi; destruct (j<=?dbi) eqn:cmpj; simpl;
+  destruct (i+d<=?dbi) eqn:cmpid; destruct (j<=?dbi+n) eqn:cmpjn; simpl;
+  destruct (i+d<=?dbi+d) eqn:cmpidd; simpl;
+  apply leb_complete in cmpj || apply leb_complete_conv in cmpj;
+  apply leb_complete in cmpi || apply leb_complete_conv in cmpi;
+  apply leb_complete in cmpjn || apply leb_complete_conv in cmpjn;
+  apply leb_complete in cmpid || apply leb_complete_conv in cmpid;
+  apply leb_complete in cmpidd || apply leb_complete_conv in cmpidd;
+  try omega; simpl.  f_equal. f_equal. omega. f_equal. f_equal. omega.
+  + assert (j<=?dbi=true) by (apply leb_correct in cmpj; assumption).
+    rewrite H. auto.
+  + assert (j<=?dbi=false) by (apply leb_correct_conv in cmpj; assumption).
+    rewrite H. auto.
+  + assert (j<=?dbi=false) by (apply leb_correct_conv in cmpj; assumption).
+    rewrite H. auto. 
+}
+all: f_equal; auto.
++ assert (i+d+1=i+1+d) by omega. rewrite H. eapply c_shift_comm_aux. omega.
++ assert (i+d+1=i+1+d) by omega. rewrite H. eapply c_shift_comm_aux. omega.
+}{
+intros cmp. induction c; simpl; f_equal; auto; 
+try eapply c_shift_comm_aux; try omega;
+assert (i+d+1=i+1+d) by omega; try rewrite H;
+assert (2=1+1) by omega; assert (i+d+(1+1)=i+(1+1)+d) by omega;
+try rewrite H0; try rewrite H1; eapply c_shift_comm_aux; omega.
+}{
+intros cmp. induction h; simpl.
+all: f_equal; auto.
+assert (2=1+1) by omega; assert (i+d+(1+1)=i+(1+1)+d) by omega;
+rewrite H; rewrite H0; eapply c_shift_comm_aux; omega.
+}
+Qed.
+
+
+Lemma v_negshift_shift (n:nat) (m:nat) (cut:nat) (v:val) :
+  (m <= n) ->
+  Sub.v_negshift (Sub.v_shift v n cut) m cut = (Sub.v_shift v (n - m) cut)
+
+with c_negshift_shift (n:nat) (m:nat) (cut:nat) (c:comp) :
+  (m <= n) ->
+  Sub.c_negshift (Sub.c_shift c n cut) m cut = (Sub.c_shift c (n - m) cut)
+
+with h_negshift_shift (n:nat) (m:nat) (cut:nat) (h:hcases) :
+  (m <= n) ->  
+  Sub.h_negshift (Sub.h_shift h n cut) m cut = (Sub.h_shift h (n - m) cut).
+Proof.
+{
+clear v_negshift_shift.  
+revert cut. induction v; intros cut m_le_n; simpl; f_equal.
+{ (* The only relevant case. *)
+  destruct v as (name, db_i). simpl.
+  induction (cut <=? db_i) eqn:cmp; simpl.
+  - apply (leb_complete _ _) in cmp.
+    assert (cut <= db_i + 1) by omega.
+    assert (cut <= db_i + n) by omega.
+    apply (leb_correct _ _) in H0. rewrite H0.
+    f_equal. f_equal. omega.
+  - rewrite cmp. reflexivity. }
+all : try reflexivity || apply IHv || apply IHv1 || apply IHv2.
+all : try apply c_negshift_shift || apply h_negshift_shift; assumption.
+}{
+clear c_negshift_shift.
+revert cut. induction c; intros cut m_le_n; try destruct p; simpl; f_equal;
+try apply v_negshift_shift || apply IHc || apply IHc1 || apply IHc2; assumption.
+}{
+clear h_negshift_shift.
+revert cut. induction h; intros cut m_le_n; simpl; f_equal.
+reflexivity. apply IHh. assumption. apply c_negshift_shift. assumption.
+}
+Qed.
+
+
+
+Lemma v_shift_0 cut v : Sub.v_shift v 0 cut = v
+with c_shift_0 cut c : Sub.c_shift c 0 cut = c
+with h_shift_0 cut h : Sub.h_shift h 0 cut = h.
+Proof.
+{
+clear v_shift_0.
+revert cut. induction v; intros cut;
+simpl; try (specialize (IHv cut)); try rewrite IHv; try reflexivity.
++ destruct v. simpl. destruct (cut <=? v0); try reflexivity.
+  assert (v0 + 0 = v0) by omega.
+  rewrite H; reflexivity.
++ rewrite IHv1, IHv2. reflexivity.
++ rewrite c_shift_0. reflexivity.
++ f_equal; try apply c_shift_0 || apply h_shift_0.
+}{
+clear c_shift_0.
+revert cut. induction c; intros cut; simpl;
+try destruct p; f_equal;
+try apply v_shift_0 || apply IHc || apply IHc1 || apply IHc2.
+}{
+clear h_shift_0.
+revert cut. induction h; intros cut; simpl; f_equal.
+reflexivity. apply IHh. apply c_shift_0.
+}
+Qed.
+
+
+Lemma v_shift_sub v v' i j (safe: j < i): 
+  Sub.v_shift (v_sub v v' j) 1 i = 
+  (v_sub (Sub.v_shift v 1 (i+1)) (Sub.v_shift v' 1 i) j)
+with c_shift_sub c v' i j (safe: j < i): 
+  Sub.c_shift (c_sub c v' j) 1 i = 
+  (c_sub (Sub.c_shift c 1 (i+1)) (Sub.v_shift v' 1 i) j)
+with h_shift_sub h v' i j (safe: j < i): 
+  Sub.h_shift (h_sub h v' j) 1 i = 
+  (h_sub (Sub.h_shift h 1 (i+1)) (Sub.v_shift v' 1 i) j).
+Proof.
+{
+induction v; unfold v_sub; simpl.
+{
+clear v_shift_sub c_shift_sub h_shift_sub.
+destruct v as (x, n). 
+destruct (n=?i) eqn:ni.
+apply Nat.eqb_eq in ni. subst.
+++ assert (i=?j=false) by (apply Nat.eqb_neq; omega).
+  rewrite H. assert (i+1<=?i=false) by (apply leb_correct_conv; omega).
+  rewrite H0. simpl. assert (j<=?i=true) by (apply leb_correct;omega).
+  rewrite H1. assert (i=?j=false) by (apply Nat.eqb_neq; omega).
+  rewrite H2. simpl. rewrite H1. assert (i<=?i-1=false).
+  apply leb_correct_conv. omega. rewrite H3. reflexivity.
+++ destruct (n=?j) eqn:nj.
++ apply Nat.eqb_eq in nj. subst.
+  assert (i+1<=?j=false) by (apply leb_correct_conv; omega).
+  rewrite H. simpl. assert (j=?j=true) by (apply Nat.eqb_eq; omega).
+  rewrite H0. rewrite v_negshift_shift. rewrite v_negshift_shift.
+  assert (1-1=0) by omega. rewrite H1. rewrite v_shift_0. rewrite v_shift_0.
+  reflexivity. omega. omega.
++ destruct (i<=?n) eqn:iln; simpl.
+  - destruct (j<=?n) eqn:jln; simpl.
+    * apply leb_complete in jln. apply leb_complete in iln.
+      assert (i<=?n-1=true).
+      { apply leb_correct. apply Nat.eqb_neq in ni. omega. }
+      rewrite H. simpl. assert (i+1<=?n=true).
+      { apply leb_correct. apply leb_complete in H. omega. }
+      rewrite H0. simpl. 
+      assert (n+1=?j=false).
+      { apply Nat.eqb_neq. omega. }
+      rewrite H1. simpl. assert (j<=?n+1=true).
+      { apply leb_correct. omega. }
+      rewrite H2. simpl.
+      f_equal. f_equal. assert (n>0) by omega. omega.
+    * rewrite iln. apply leb_complete in iln. assert (i+1<=?n=true).
+      { apply leb_correct. apply Nat.eqb_neq in ni. omega. }
+      rewrite H. apply leb_complete in H. apply leb_complete_conv in jln. omega. 
+  - apply leb_complete_conv in iln.
+    assert (i+1<=?n=false) by (apply leb_correct_conv; omega).
+    rewrite H. simpl. rewrite nj. simpl.
+    destruct (j<=?n) eqn:jln.
+    * simpl. assert (i<=?n-1=false).
+      { apply leb_correct_conv. omega. }
+      rewrite H0. reflexivity.
+    * simpl. assert (i<=?n=false) by (apply leb_correct_conv; omega).
+      rewrite H0. reflexivity.
+}     
+all: f_equal; auto.
++ clear v_shift_sub h_shift_sub.
+  unfold c_sub in c_shift_sub. rewrite v_shift_comm_aux. rewrite c_shift_sub.
+  f_equal. f_equal. f_equal. rewrite (v_shift_comm_aux 1 j). f_equal.
+  rewrite (v_shift_comm_aux 1 i). f_equal. all: omega.
++ clear v_shift_sub h_shift_sub.
+  unfold c_sub in c_shift_sub. rewrite v_shift_comm_aux. rewrite c_shift_sub.
+  f_equal. f_equal. f_equal. rewrite (v_shift_comm_aux 1 j). f_equal.
+  rewrite (v_shift_comm_aux 1 i). f_equal. all: omega.
++ apply h_shift_sub. auto.
+}{
+induction c; unfold c_sub; simpl; f_equal;
+try apply v_shift_sub; try assumption.
++ clear v_shift_sub h_shift_sub.
+  unfold c_sub in c_shift_sub. rewrite <-(v_shift_shift 1).
+  rewrite (v_shift_comm_aux 1 j). rewrite (v_shift_comm_aux 1 (j+1)).
+  assert (j+1+1=j+2) by omega. rewrite H. rewrite c_shift_sub. clear c_shift_sub.
+  f_equal. f_equal. f_equal. all: try omega.
+  rewrite <-(v_shift_shift 1 1 0). rewrite (v_shift_comm_aux 1 j).
+  rewrite (v_shift_comm_aux 1 (j+1)). f_equal. rewrite (v_shift_comm_aux 1 i).
+  rewrite (v_shift_comm_aux 1 (i+1)). f_equal. f_equal. all: omega.
++ clear v_shift_sub h_shift_sub.
+  unfold c_sub in c_shift_sub. rewrite v_shift_comm_aux. rewrite c_shift_sub.
+  f_equal. f_equal. f_equal. rewrite (v_shift_comm_aux 1 j). f_equal.
+  rewrite (v_shift_comm_aux 1 i). f_equal. all: omega.
++ clear v_shift_sub h_shift_sub.
+  unfold c_sub in c_shift_sub. rewrite v_shift_comm_aux. rewrite c_shift_sub.
+  f_equal. f_equal. f_equal. rewrite (v_shift_comm_aux 1 j). f_equal.
+  rewrite (v_shift_comm_aux 1 i). f_equal. all: omega.
++ clear v_shift_sub h_shift_sub.
+  unfold c_sub in c_shift_sub. rewrite v_shift_comm_aux. rewrite c_shift_sub.
+  f_equal. f_equal. f_equal. rewrite (v_shift_comm_aux 1 j). f_equal.
+  rewrite (v_shift_comm_aux 1 i). f_equal. all: omega.
++ clear v_shift_sub h_shift_sub.
+  unfold c_sub in c_shift_sub. rewrite <-(v_shift_shift 1).
+  rewrite (v_shift_comm_aux 1 j). rewrite (v_shift_comm_aux 1 (j+1)).
+  assert (j+1+1=j+2) by omega. rewrite H. rewrite c_shift_sub. clear c_shift_sub.
+  f_equal. f_equal. f_equal. all: try omega.
+  rewrite <-(v_shift_shift 1 1 0). rewrite (v_shift_comm_aux 1 j).
+  rewrite (v_shift_comm_aux 1 (j+1)). f_equal. rewrite (v_shift_comm_aux 1 i).
+  rewrite (v_shift_comm_aux 1 (i+1)). f_equal. f_equal. all: omega.
++ clear v_shift_sub h_shift_sub.
+  unfold c_sub in c_shift_sub. rewrite v_shift_comm_aux. rewrite c_shift_sub.
+  f_equal. f_equal. f_equal. rewrite (v_shift_comm_aux 1 j). f_equal.
+  rewrite (v_shift_comm_aux 1 i). f_equal. all: omega.
++ clear v_shift_sub h_shift_sub.
+  unfold c_sub in c_shift_sub. rewrite v_shift_comm_aux. rewrite c_shift_sub.
+  f_equal. f_equal. f_equal. rewrite (v_shift_comm_aux 1 j). f_equal.
+  rewrite (v_shift_comm_aux 1 i). f_equal. all: omega.
+}{
+induction h; unfold h_sub; simpl. auto. f_equal.
++ apply h_shift_sub. assumption.
++ clear v_shift_sub h_shift_sub.
+  unfold c_sub in c_shift_sub. rewrite <-(v_shift_shift 1).
+  rewrite (v_shift_comm_aux 1 j). rewrite (v_shift_comm_aux 1 (j+1)).
+  assert (j+1+1=j+2) by omega. rewrite H. rewrite c_shift_sub. clear c_shift_sub.
+  f_equal. f_equal. f_equal. all: try omega.
+  rewrite <-(v_shift_shift 1 1 0). rewrite (v_shift_comm_aux 1 j).
+  rewrite (v_shift_comm_aux 1 (j+1)). f_equal. rewrite (v_shift_comm_aux 1 i).
+  rewrite (v_shift_comm_aux 1 (i+1)). f_equal. f_equal. all: omega.
+}
+Qed.
+
+
+(* 
+Lemma v_shift_sub v v' i j (safe: i < j): 
+  Sub.v_shift (v_sub v v' j) 1 i = 
+  (v_sub (Sub.v_shift v 1 i) (Sub.v_shift v' 1 i) (j+1))
+with c_shift_sub c v' i j (safe: i < j): 
+  Sub.c_shift (c_sub c v' j) 1 i = 
+  (c_sub (Sub.c_shift c 1 i) (Sub.v_shift v' 1 i) (j+1))
+with h_shift_sub h v' i j (safe: i < j): 
+  Sub.h_shift (h_sub h v' j) 1 i = 
+  (h_sub (Sub.h_shift h 1 i) (Sub.v_shift v' 1 i) (j+1)).
+Proof.
+{
+induction v; unfold v_sub; simpl.
+{
+clear v_shift_sub c_shift_sub h_shift_sub.
+destruct v as (x, n). destruct (n=?j) eqn:nj.
++ apply Nat.eqb_eq in nj. subst.
+  assert (i<=?j=true) by (apply leb_correct; omega).
+  rewrite H. simpl. assert (j+1=?j+1=true) by (apply Nat.eqb_eq; omega).
+  rewrite H0. rewrite v_negshift_shift. rewrite v_negshift_shift.
+  assert (1-1=0) by omega. rewrite H1. rewrite v_shift_0. rewrite v_shift_0.
+  reflexivity. omega. omega.
++ destruct (i<=?n) eqn:iln; simpl.
+  - destruct (j<=?n) eqn:jln; simpl.
+    * assert (i<=?n-1=true). all: apply leb_complete in jln.
+      { apply leb_complete in iln. 
+        apply leb_correct. omega. }
+      rewrite H. assert (n+1=?j+1=false).
+      { apply Nat.eqb_neq. apply Nat.eqb_neq in nj. omega. }
+      rewrite H0. simpl. assert (j+1<=?n+1=true).
+      { apply leb_correct. omega. }
+      rewrite H1. f_equal. f_equal. assert (n>0) by omega. omega.
+    * rewrite iln. assert (n+1=?j+1=false).
+      { apply Nat.eqb_neq. apply Nat.eqb_neq in nj. omega. }
+      rewrite H. simpl. assert (j+1<=?n+1=false).
+      { apply leb_correct_conv. apply leb_complete_conv in jln. omega. }
+      rewrite H0. reflexivity.
+  - apply leb_complete_conv in iln. apply Nat.eqb_neq in nj.
+    assert (j<=?n=false) by (apply leb_correct_conv; omega).
+    rewrite H. assert (n=?j+1=false) by (apply Nat.eqb_neq; omega).
+    rewrite H0. simpl. assert (i<=?n=false) by (apply leb_correct_conv;omega).
+    rewrite H1. assert (j+1<=?n=false) by (apply leb_correct_conv; omega).
+    rewrite H2. reflexivity.
+}     
+all: f_equal; auto.
++ clear v_shift_sub h_shift_sub.
+  unfold c_sub in c_shift_sub. rewrite v_shift_comm_aux. rewrite c_shift_sub.
+  f_equal. f_equal. f_equal. rewrite (v_shift_comm_aux 1 (j+1)). f_equal.
+  rewrite (v_shift_comm_aux 1 i). f_equal. all: omega.
++ clear v_shift_sub h_shift_sub.
+  unfold c_sub in c_shift_sub. rewrite v_shift_comm_aux. rewrite c_shift_sub.
+  f_equal. f_equal. f_equal. rewrite (v_shift_comm_aux 1 (j+1)). f_equal.
+  rewrite (v_shift_comm_aux 1 i). f_equal. all: omega.
++ apply h_shift_sub. auto.
+}{
+induction c; unfold c_sub; simpl; f_equal;
+try apply v_shift_sub; try assumption.
++ clear v_shift_sub h_shift_sub.
+  unfold c_sub in c_shift_sub. rewrite <-(v_shift_shift 1).
+  rewrite (v_shift_comm_aux 1 j). rewrite (v_shift_comm_aux 1 (j+1)).
+  assert (j+1+1=j+2) by omega. rewrite H. rewrite c_shift_sub. clear c_shift_sub.
+  f_equal. f_equal. f_equal. all: try omega.
+  rewrite <-(v_shift_shift 1 1 0). rewrite (v_shift_comm_aux 1 (j+1)).
+  rewrite (v_shift_comm_aux 1 (j+1+1)). f_equal. rewrite (v_shift_comm_aux 1 i).
+  rewrite (v_shift_comm_aux 1 (i+1)). f_equal. all: omega.
++ clear v_shift_sub h_shift_sub.
+  unfold c_sub in c_shift_sub. rewrite v_shift_comm_aux. rewrite c_shift_sub.
+  f_equal. f_equal. f_equal. rewrite (v_shift_comm_aux 1 (j+1)). f_equal.
+  rewrite (v_shift_comm_aux 1 i). f_equal. all: omega.
++ clear v_shift_sub h_shift_sub.
+  unfold c_sub in c_shift_sub. rewrite v_shift_comm_aux. rewrite c_shift_sub.
+  f_equal. f_equal. f_equal. rewrite (v_shift_comm_aux 1 (j+1)). f_equal.
+  rewrite (v_shift_comm_aux 1 i). f_equal. all: omega.
++ clear v_shift_sub h_shift_sub.
+  unfold c_sub in c_shift_sub. rewrite v_shift_comm_aux. rewrite c_shift_sub.
+  f_equal. f_equal. f_equal. rewrite (v_shift_comm_aux 1 (j+1)). f_equal.
+  rewrite (v_shift_comm_aux 1 i). f_equal. all: omega.
++ clear v_shift_sub h_shift_sub.
+  unfold c_sub in c_shift_sub. rewrite <-(v_shift_shift 1).
+  rewrite (v_shift_comm_aux 1 j). rewrite (v_shift_comm_aux 1 (j+1)).
+  assert (j+1+1=j+2) by omega. rewrite H. rewrite c_shift_sub. clear c_shift_sub.
+  f_equal. f_equal. f_equal. all: try omega.
+  rewrite <-(v_shift_shift 1 1 0). rewrite (v_shift_comm_aux 1 (j+1)).
+  rewrite (v_shift_comm_aux 1 (j+1+1)). f_equal. rewrite (v_shift_comm_aux 1 i).
+  rewrite (v_shift_comm_aux 1 (i+1)). f_equal. all: omega.
++ clear v_shift_sub h_shift_sub.
+  unfold c_sub in c_shift_sub. rewrite v_shift_comm_aux. rewrite c_shift_sub.
+  f_equal. f_equal. f_equal. rewrite (v_shift_comm_aux 1 (j+1)). f_equal.
+  rewrite (v_shift_comm_aux 1 i). f_equal. all: omega.
++ clear v_shift_sub h_shift_sub.
+  unfold c_sub in c_shift_sub. rewrite v_shift_comm_aux. rewrite c_shift_sub.
+  f_equal. f_equal. f_equal. rewrite (v_shift_comm_aux 1 (j+1)). f_equal.
+  rewrite (v_shift_comm_aux 1 i). f_equal. all: omega.
+}{
+induction h; unfold h_sub; simpl. auto. f_equal.
++ apply h_shift_sub. assumption.
++ clear v_shift_sub h_shift_sub.
+  unfold c_sub in c_shift_sub. rewrite <-(v_shift_shift 1).
+  rewrite (v_shift_comm_aux 1 j). rewrite (v_shift_comm_aux 1 (j+1)).
+  assert (j+1+1=j+2) by omega. rewrite H. rewrite c_shift_sub. clear c_shift_sub.
+  f_equal. f_equal. f_equal. all: try omega.
+  rewrite <-(v_shift_shift 1 1 0). rewrite (v_shift_comm_aux 1 (j+1)).
+  rewrite (v_shift_comm_aux 1 (j+1+1)). f_equal. rewrite (v_shift_comm_aux 1 i).
+  rewrite (v_shift_comm_aux 1 (i+1)). f_equal. all: omega.
+}
+Qed.
+
+
+
+ *)
