language_formalisation/syntax/syntax_lemmas.v
@@ -1,5 +1,5 @@
-Add LoadPath "C:\Users\Ziga\Documents\Ziga_podatki\PHD\language_formalisation\syntax".
-(* Add LoadPath "E:\Ziga_Podatki\faks\PHD\language_formalisation\syntax". *)
+(* Add LoadPath "C:\Users\Ziga\Documents\Ziga_podatki\PHD\language_formalisation\syntax". *)
+Add LoadPath "E:\Ziga_Podatki\faks\PHD\language_formalisation\syntax".
 Require Export Arith syntax.
 Require Import Le Compare_dec.
 
@@ -10,9 +10,7 @@ Lemma get_ctx_remove_unchanged Γ i j :
   i > j -> get_vtype Γ j = get_vtype (ctx_remove_var Γ i) j.
 Proof.
 revert i j; induction Γ; intros i j lt; auto.
-destruct i; destruct j; simpl.
-+ omega.
-+ omega.
+destruct i; destruct j; simpl; try omega.
 + reflexivity.
 + apply IHΓ. omega.
 Qed.
@@ -27,11 +25,13 @@ destruct i; destruct j; simpl; auto.
 + apply IHΓ. omega.
 Qed.
 
+
 Lemma ctx_remove_extend Γ i A :
   CtxU (ctx_remove_var Γ i) A = ctx_remove_var (CtxU Γ A) (i+1).
 Proof.
 revert i; induction Γ; intros i; assert (i+1 = S i) by omega; rewrite H; auto.
 Qed.
+
 
 Lemma get_ctx_insert_unchanged Γ A i j:
   i < j -> get_vtype Γ i = get_vtype (ctx_insert_var Γ A j) i.
@@ -43,6 +43,7 @@ destruct i; destruct j; simpl; try reflexivity.
   - omega.
   - simpl. destruct i; auto. apply IHΓ. omega.
 Qed.
+
 
 Lemma get_ctx_insert_changed Γ A i j:
   i >= j -> get_vtype Γ i = get_vtype (ctx_insert_var Γ A j) (i+1).
@@ -56,11 +57,13 @@ destruct j; destruct i.
 + simpl. apply IHΓ. omega.
 Qed.
 
+
 Lemma ctx_insert_extend Γ i A_ins A :
   CtxU (ctx_insert_var Γ A_ins i) A = ctx_insert_var (CtxU Γ A) A_ins (i+1).
 Proof.
 revert i; induction Γ; intros i; assert (i+1 = S i) by omega; rewrite H; auto.
 Qed.
+
 
 Lemma join_ctxs_insert_var Γ1 Γ2 i A :
   join_ctxs (ctx_insert_var Γ1 A i) Γ2= 
@@ -71,6 +74,7 @@ assert (i + S (ctx_len Γ2) = S (i + ctx_len Γ2)) by omega.
 rewrite H. f_equal. auto.
 Qed.
 
+
 Lemma join_ctx_tctx_insert_var  Γ Z D i A :
   join_ctx_tctx (ctx_insert_var Γ A i) Z D = 
     ctx_insert_var (join_ctx_tctx Γ Z D) A (i + tctx_len Z). 
@@ -79,6 +83,7 @@ induction Z; simpl. auto.
 assert (i + S (tctx_len Z) = S (i + tctx_len Z)) by omega.
 rewrite H. f_equal. auto.
 Qed.
+
 
 Lemma ctx_len_get_vtype Γ n :
   (exists A, get_vtype Γ n = Some A) <-> ctx_len Γ > n.
@@ -96,11 +101,13 @@ constructor.
     * apply IHΓ. omega.
 Qed.
 
+
 Lemma ctx_len_gets Γ n A:
   get_vtype Γ n = Some A -> ctx_len Γ > n.
 Proof.
 intro. apply ctx_len_get_vtype. eauto.
 Qed.
+
 
 Lemma tctx_len_get_ttype Z n :
   (exists A, get_ttype Z n = Some A) <-> tctx_len Z > n.
@@ -117,6 +124,7 @@ constructor.
     * eauto.
     * apply IHZ. omega.
 Qed.
+
 
 Lemma tctx_len_gets Z n A:
   get_ttype Z n = Some A -> tctx_len Z > n.
